Lots of refactoring: new directory structure for heaps and BSTs, changed most definitions of counting functions, moved lazy lists to trash, factored out an 'Enhanced Binary Tree' type which is then reused by redblack trees and height balanced trees, renamed Basic/ to Data/, Set to FinSet, improved automation a bit.

DS/BST/RedBlack.v
@@ -2,72 +2,54 @@ Require Export RCCBase.
 
 Require Export BTree.
 Require Export TrichDec.
-Require Export Sorting.Sort.
+
+Require Export EBTree.
 
 Inductive color : Set :=
     | Red : color
     | Black : color.
 
-Inductive RBTree (A : Type) : Type :=
-    | E : RBTree A
-    | T : color -> RBTree A -> A -> RBTree A -> RBTree A.
-
-Arguments E {A}.
-Arguments T {A} _ _ _.
-
-Inductive Elem {A : Type} (x : A) : RBTree A -> Prop :=
-    | Elem_root : forall (c : color) (l r : RBTree A),
-        Elem x (T c l x r)
-    | Elem_left : forall (c : color) (v : A) (l r : RBTree A),
-        Elem x l -> Elem x (T c l v r)
-    | Elem_right : forall  (c : color) (v : A) (l r : RBTree A),
-        Elem x r -> Elem x (T c l v r).
+Definition RBTree (A : Type) : Type := EBTree color A.
 
 Inductive isBST {A : TrichDec} : RBTree A -> Prop :=
     | isBST_E : isBST E
     | isBST_T : forall (c : color) (v : A) (l r : RBTree A),
         (forall x : A, Elem x l -> x ≤ v) -> isBST l ->
         (forall x : A, Elem x r -> v ≤ x) -> isBST r ->
-        isBST (T c l v r).
+        isBST (N c l v r).
 
-Hint Constructors color RBTree Elem isBST : core.
+Hint Constructors color EBTree Elem isBST : core.
 
 (** [empty], [isEmpty] and [singleton] are my own. *)
 Definition empty {A : Type} : RBTree A := E.
 
-Definition isEmpty {A : Type} (t : RBTree A) : bool :=
-match t with
-    | E => true
-    | _ => false
-end.
-
-Definition singleton {A : Type} (x : A) : RBTree A := T Red E x E.
+Definition singleton {A : Type} (x : A) : RBTree A := N Red E x E.
 
 Function balance {A : Type} (c : color)
   (l : RBTree A) (v : A) (r : RBTree A) : RBTree A :=
 match c with
-    | Red => T Red l v r
+    | Red => N Red l v r
     | Black =>
         match l, v, r with
-            | T Red (T Red a xv b) yv c, zv, d
-            | T Red a xv (T Red b yv c), zv, d
-            | a, xv, T Red (T Red b yv c) zv d
-            | a, xv, T Red b yv (T Red c zv d) =>
-                T Red (T Black a xv b) yv (T Black c zv d)
-            | l, v, r => T Black l v r
+            | N Red (N Red a xv b) yv c, zv, d
+            | N Red a xv (N Red b yv c), zv, d
+            | a, xv, N Red (N Red b yv c) zv d
+            | a, xv, N Red b yv (N Red c zv d) =>
+                N Red (N Black a xv b) yv (N Black c zv d)
+            | l, v, r => N Black l v r
         end
 end.
 
 Definition makeBlack {A : Type} (t : RBTree A) :=
 match t with
     | E => E
-    | T _ l v r => T Black l v r
+    | N _ l v r => N Black l v r
 end.
 
 Function ins {A : TrichDec} (x : A) (t : RBTree A) : RBTree A :=
 match t with
-    | E => T Red E x E
-    | T c l v r =>
+    | E => N Red E x E
+    | N c l v r =>
         if x ≤? v
         then balance c (ins x l) v r
         else balance c l v (ins x r)
@@ -75,19 +57,6 @@ end.
 
 Definition insert {A : TrichDec} (x : A) (t : RBTree A) : RBTree A :=
   makeBlack (ins x t).
-
-Fixpoint countRBT {A : Type} (p : A -> bool) (t : RBTree A) : nat :=
-match t with
-    | E => 0
-    | T _ l v r =>
-        (if p v then S else id) (countRBT p l + countRBT p r)
-end.
-
-Function toList {A : Type} (t : RBTree A) : list A :=
-match t with
-    | E => []
-    | T _ l v r => toList l ++ v :: toList r
-end.
 
 Fixpoint fromList {A : TrichDec} (l : list A) : RBTree A :=
 match l with
@@ -155,7 +124,7 @@ Qed.
 
 Lemma Elem_inv :
   forall (A : Type) (P : A -> Prop) (c : color) (v : A) (l r : RBTree A),
-    (forall x : A, Elem x (T c l v r) -> P x) ->
+    (forall x : A, Elem x (N c l v r) -> P x) ->
       P v /\
       (forall x : A, Elem x l -> P x) /\
       (forall x : A, Elem x r -> P x).
@@ -163,7 +132,7 @@ Proof.
   repeat split; intros; apply H; auto.
 Qed.
 
-Lemma trich_le_trans :
+(* Lemma trich_le_trans :
   forall {A : TrichDec} {x y z : A},
     x ≤ y -> y ≤ z -> x ≤ z.
 Proof.
@@ -174,6 +143,7 @@ Proof.
     subst. left. assumption.
     subst. apply trich_le_refl.
 Qed.
+ *)
 
 Ltac aux := intros;
 repeat match goal with
@@ -183,15 +153,15 @@ try match goal with
     | H : False |- _ => destruct H
 end;
 repeat match goal with
-    | H : isBST (T _ _ _ _) |- _ => inv H
+    | H : isBST (N _ _ _ _) |- _ => inv H
     | H : Elem _ E |- _ => destruct H
-    | H : Elem _ (T _ _ _ _) |- _ => inv H
+    | H : Elem _ (N _ _ _ _) |- _ => inv H
     | |- isBST _ => constructor; auto
     | |- forall _, Elem _ _ -> _ => inv 1
 end;
 repeat match goal with
     | H : _ /\ _ |- _ => destruct H
-    | H : forall _, Elem _ (T _ _ _ _) -> _ |- _ =>
+    | H : forall _, Elem _ (N _ _ _ _) -> _ |- _ =>
         apply Elem_inv in H
 end;
 repeat match goal with
@@ -206,14 +176,14 @@ end. *)
 
 Lemma Elem_balance :
   forall (A : TrichDec) (c : color) (x v : A) (l r : RBTree A),
-    Elem x (T c l v r) <-> Elem x (balance c l v r).
+    Elem x (N c l v r) <-> Elem x (balance c l v r).
 Proof.
   split; functional induction @balance (@carrier A) c l v r; aux.
 Qed.
 
 Lemma isBST_balance :
   forall (A : TrichDec) (c : color) (v : A) (l r : RBTree A),
-    isBST (T c l v r) -> isBST (balance c l v r).
+    isBST (N c l v r) -> isBST (balance c l v r).
 Proof.
   intros.
   functional induction balance c l v r; aux; trich.
@@ -224,9 +194,9 @@ match goal with
     | |- context [if ?p then _ else _] => destruct p
 end.
 
-Lemma countRBT_balance :
+Lemma countEBT_balance :
   forall (A : Type) (p : A -> bool) (c : color) (v : A) (l r : RBTree A),
-    countRBT p (balance c l v r) = countRBT p (T c l v r).
+    countEBT p (balance c l v r) = countEBT p (N c l v r).
 Proof.
   intros. functional induction @balance A c l v r;
   cbn; destruct_if;
@@ -249,9 +219,9 @@ Proof.
   destruct t; cbn; inv 1.
 Qed.
 
-Lemma makeBlack_countRBT :
+Lemma countEBT_makeBlack :
   forall (A : Type) (p : A -> bool) (t : RBTree A),
-    countRBT p (makeBlack t) = countRBT p t.
+    countEBT p (makeBlack t) = countEBT p t.
 Proof.
   destruct t; reflexivity.
 Qed.
@@ -269,6 +239,11 @@ Proof.
     induction t; cbn; intros.
       inv H.
       trich; rewrite <- Elem_balance; inv H; inv H1.
+Restart.
+  intros until t. revert x.
+  functional induction ins y t;
+  intros; rewrite <- ?Elem_balance, ?Elem_N, ?IHl, ?IHr;
+  firstorder.
 Qed.
 
 Lemma isBST_ins :
@@ -283,12 +258,12 @@ Proof.
       intros. rewrite Elem_ins in H. inv H. trich.
 Qed.
 
-Lemma countRBT_ins :
+Lemma countEBT_ins :
   forall (A : TrichDec) (p : A -> bool) (x : A) (t : RBTree A),
-    countRBT p (ins x t) = (if p x then S else id) (countRBT p t).
+    countEBT p (ins x t) = (if p x then 1 else 0) + countEBT p t.
 Proof.
   induction t; cbn; trich;
-  rewrite countRBT_balance; cbn; rewrite ?IHt1, ?IHt2;
+  rewrite countEBT_balance; cbn; rewrite ?IHt1, ?IHt2;
   destruct_if; unfold id; lia.
 Qed.
 
@@ -308,17 +283,17 @@ Proof.
   intros. unfold insert. apply isBST_makeBlack, isBST_ins. assumption.
 Qed.
 
-Lemma countRBT_insert :
+Lemma countEBT_insert :
   forall (A : TrichDec) (p : A -> bool) (x : A) (t : RBTree A),
-    countRBT p (insert x t) = (if p x then S else id) (countRBT p t).
+    countEBT p (insert x t) = (if p x then 1 else 0) + countEBT p t.
 Proof.
   intros. unfold insert.
-  rewrite makeBlack_countRBT, countRBT_ins. reflexivity.
+  rewrite countEBT_makeBlack, countEBT_ins. reflexivity.
 Qed.
 
 Lemma Permutation_toList_balance :
   forall (A : Type) (c : color) (v : A) (l r : RBTree A),
-    Permutation (toList (balance c l v r)) (toList (T c l v r)).
+    Permutation (toList (balance c l v r)) (toList (N c l v r)).
 Proof.
   intros.
   functional induction balance c l v r;
@@ -345,8 +320,8 @@ Lemma Permutation_toList_insert :
     Permutation (toList (insert x t)) (x :: toList t).
 Proof.
   intros. unfold insert. destruct (ins x t) eqn: Heq; cbn.
-    apply (f_equal (countRBT (fun _ => true))) in Heq.
-      rewrite countRBT_ins in Heq. cbn in Heq. inv Heq.
+    apply (f_equal (countEBT (fun _ => true))) in Heq.
+      rewrite countEBT_ins in Heq. cbn in Heq. inv Heq.
     rewrite <- (Permutation_toList_ins _ x t). rewrite Heq.
       cbn. reflexivity.
 Qed.
@@ -363,14 +338,16 @@ Proof.
     induction 1; cbn; apply in_or_app; firstorder.
 Qed.
 
-Lemma toList_countRBT :
+Require Export Sorting.Sort.
+
+Lemma toList_countEBT :
   forall (A : Type) (p : A -> bool) (t : RBTree A),
-    countRBT p t = count p (toList t).
+    countEBT p t = count p (toList t).
 Proof.
   induction t; cbn.
     reflexivity.
     rewrite count_app, IHt1, IHt2.
-      cbn. destruct (p a); auto.
+      cbn. destruct (p a); lia.
 Qed.
 
 Lemma Sorted_toList :
@@ -410,12 +387,12 @@ Proof.
     apply isBST_insert. assumption.
 Qed.
 
-Lemma countRBT_fromList :
+Lemma countEBT_fromList :
   forall (A : TrichDec) (p : A -> bool) (l : list A),
-    countRBT p (fromList l) = count p l.
+    countEBT p (fromList l) = count p l.
 Proof.
   induction l as [| h t]; cbn; trich;
-  rewrite countRBT_insert, IHt.
+  rewrite countEBT_insert, IHt.
   destruct (p h); reflexivity.
 Qed.
 
@@ -433,7 +410,7 @@ Lemma perm_redblackSort :
     perm l (redblackSort A l).
 Proof.
   unfold perm, redblackSort. intros.
-  rewrite <- toList_countRBT, countRBT_fromList. reflexivity.
+  rewrite <- toList_countEBT, countEBT_fromList. reflexivity.
 Qed.
 
 Lemma Permutation_redblackSort :
