DS/BST/HeightBalanced.v
@@ -1,0 +1,80 @@
+Require Export RCCBase.
+Require Export TrichDec.
+Require Export Data.EBTree.
+
+Definition Tree (A : Type) : Type := EBTree nat A.
+
+Definition height' {A : Type} (t : Tree A) : nat :=
+match t with
+    | E => 0
+    | N h _ _ _ => h
+end.
+
+Definition balance {A : Type} (l : Tree A) (v : A) (r : Tree A) : Tree A :=
+  N (1 + max (height l) (height r)) l v r.
+
+Function rotateLR {A : Type} (t : Tree A) : Tree A :=
+match t with
+    | N _ (N _ a y b) x c => balance a y (balance b x c)
+    | _ => t
+end.
+
+Function rotateRL {A : Type} (t : Tree A) : Tree A :=
+match t with
+    | N _ a x (N _ b y c) => balance (balance a x b) y c
+    | _ => t
+end.
+
+Function rebalance {A : Type} (l : Tree A) (v : A) (r : Tree A) : Tree A :=
+match height l <?> height r with
+    | Lt =>
+        match r with
+            | N _ a x b => balance (balance l x a) v b
+            | _ => balance l v r
+        end
+    | Eq => balance l v r
+    | Gt =>
+        match l with
+            | N _ a x b => balance a v (balance b x r)
+            | _ => balance l v r
+        end
+end.
+
+Function insert {A : TrichDec} (x : A) (t : Tree A) : Tree A :=
+match t with
+    | E => N 1 E x E
+    | N _ l v r =>
+        if x ≤? v
+        then rebalance (insert x l) v r
+        else rebalance l v (insert x r)
+end.
+
+Lemma height_balance :
+  forall (A : Type) (v : A) (l r : Tree A),
+    height (balance l v r) = 1 + max (height l) (height r).
+Proof.
+  cbn. reflexivity.
+Qed.
+
+(* TODO: height_rotate *)
+
+Lemma height_rebalance :
+  forall (A : Type) (v : A) (l r : Tree A),
+    height (rebalance l v r) <= 1 + max (height l) (height r).
+Proof.
+  intros. functional induction @rebalance A l v r; trich; cbn in *.
+    destruct (height b).
+      rewrite (@cmp_spec1 natlt) in e. cbn in e. lia.
+      rewrite (@cmp_spec1 natlt) in e. cbn in e. lia.
+    destruct (height r).
+      rewrite (@cmp_spec1 natlt) in e. cbn in e. lia.
+      rewrite (@cmp_spec1 natlt) in e. cbn in e. lia.
+Qed.
+
+Lemma height_insert :
+  forall (A : TrichDec) (x : A) (t : Tree A),
+    height (insert x t) <= 1 + height t.
+Proof.
+  intros. functional induction insert x t;
+  cbn; rewrite ?height_rebalance; lia.
+Qed.
