Data/EBTree.v
@@ -1,0 +1,63 @@
+Require Export RCCBase.
+
+Inductive EBTree (M A : Type) : Type :=
+    | E : EBTree M A
+    | N : M -> EBTree M A -> A -> EBTree M A -> EBTree M A.
+
+Arguments E {M A}.
+Arguments N {M A} _ _ _ _.
+
+Inductive Elem {M A : Type} (x : A) : EBTree M A -> Prop :=
+    | Elem_root :
+        forall (m : M) (l r : EBTree M A),
+        Elem x (N m l x r)
+    | Elem_left :
+        forall (m : M) (v : A) (l r : EBTree M A),
+        Elem x l -> Elem x (N m l v r)
+    | Elem_right :
+        forall (m : M) (v : A) (l r : EBTree M A),
+        Elem x r -> Elem x (N m l v r).
+
+Hint Constructors EBTree Elem : core.
+
+Lemma Elem_N :
+  forall {M A : Type} (m : M) (x v : A) (l r : EBTree M A),
+    Elem x (N m l v r) <-> x = v \/ Elem x l \/ Elem x r.
+Proof.
+  split; inv 1. inv H0.
+Qed.
+
+(* 
+
+Inductive isBST {A : TrichDec} : EBTree M A -> Prop :=
+    | isBST_E : isBST E
+    | isBST_T : forall (c : color) (v : A) (l r : EBTree M A),
+        (forall x : A, Elem x l -> x ≤ v) -> isBST l ->
+        (forall x : A, Elem x r -> v ≤ x) -> isBST r ->
+        isBST (T c l v r). *)
+
+Definition isEmpty {M A : Type} (t : EBTree M A) : bool :=
+match t with
+    | E => true
+    | _ => false
+end.
+
+Fixpoint height {M A : Type} (t : EBTree M A) : nat :=
+match t with
+    | E => 0
+    | N _ l _ r => 1 + max (height l) (height r)
+end.
+
+Function toList {M A : Type} (t : EBTree M A) : list A :=
+match t with
+    | E => []
+    | N _ l v r => toList l ++ v :: toList r
+end.
+
+Fixpoint countEBT {M A : Type} (p : A -> bool) (t : EBTree M A) : nat :=
+match t with
+    | E => 0
+    | N _ l v r =>
+(*         (if p v then S else id) (countEBT p l + countEBT p r) *)
+        (if p v then 1 else 0) + countEBT p l + countEBT p r
+end.
